spot/GC.SPOT.HeapExpansion.fst
@@ -1861,6 +1861,13 @@ let spot_chunked_promote_object_head_split_preserves_chunked_alloc_shape
           (forall (src:obj_addr).
             Seq.mem src (MH.major_objects mh) ==>
             Seq.mem src (MH.major_objects res.major_out)) /\
+          (forall (src:obj_addr). forall (hdr:U64.t).
+            Seq.mem src (MH.major_objects mh) /\
+            src <> fp /\
+            MH.read_word_in_major mh (hd_address src) == Some hdr /\
+            U64.v (Obj.getWosize hdr) >= 1 ==>
+            MH.read_word_in_major res.major_out (hd_address src) ==
+              Some hdr) /\
           Seq.mem (fp <: obj_addr)
             (MH.major_objects alloc_res.major_alloc_out) /\
           Seq.mem (fp <: obj_addr) (MH.major_objects res.major_out))))
@@ -1892,6 +1899,31 @@ let spot_chunked_promote_object_head_split_preserves_chain_objects_blue
   =
   CheneyPreservation.chunked_promote_object_head_split_preserves_chain_objects_blue
     minor mh obj fp wosize fuel
+
+let spot_chunked_promote_object_head_split_preserves_old_non_blue_header
+  (minor: minor_state) (mh: MH.major_heap) (obj: U64.t)
+  (fp: U64.t) (wosize: nat{wosize > 0}) (fuel: nat)
+  (src: obj_addr) (hdr: U64.t)
+  : Lemma
+      (requires
+        fuel > 1 /\
+        fp <> 0UL /\
+        GenInv.chunked_major_alloc_shape mh fp fuel /\
+        SpecMajorAlloc.major_fl_chain_terminates mh fp fuel = true /\
+        GenInv.chunked_chain_objects_blue mh fp fuel /\
+        SpecMajorAlloc.major_fl_head_wosize mh fp >= wosize + 2 /\
+        Seq.mem src (MH.major_objects mh) /\
+        MH.read_word_in_major mh (hd_address src) == Some hdr /\
+        Obj.getColor hdr <> GC.Lib.Header.Blue /\
+        U64.v (Obj.getWosize hdr) >= 1)
+      (ensures
+        (let res =
+           ChunkedPromote.chunked_promote_object_with_fuel
+             minor mh obj fp wosize fuel in
+         MH.read_word_in_major res.major_out (hd_address src) == Some hdr))
+  =
+  CheneyPreservation.chunked_promote_object_head_split_preserves_old_non_blue_header
+    minor mh obj fp wosize fuel src hdr
 
 let spot_chunked_promote_object_head_split_preserves_remaining_head_wosize
   (minor: minor_state) (mh: MH.major_heap) (obj: U64.t)
